fairness/lm_fair.v
@@ -3,6 +3,111 @@ From trillium.fairness Require Import fairness fuel fuel_ext utils.
 Close Scope Z_scope.
 
 
+Section LocaleTrans.
+  Context `{LM: LiveModel G M LSI}. 
+  Context `{Countable G}.
+  Context `{∀ s1 ρ s2, Decision (fmtrans M s1 (Some ρ) s2)}.
+  Context `{EqDecision (fmstate M)}. 
+
+  (* TODO: rename *)
+  Definition locale_trans  (st1: lm_ls LM) (τ: G) st2 :=
+    exists ℓ, ls_trans (lm_fl LM) st1 ℓ st2 /\ fair_lbl_matches_group ℓ τ. 
+    
+  Definition potential_step_FLs `{LM: LiveModel G M LSI}
+    (st1: lm_ls LM) (τ: G): 
+    gset (@FairLabel G (fmrole M)) :=
+    {[ Silent_step τ ]} ∪ (set_map (fun ρ => Take_step ρ τ) (dom (ls_fuel st1))).
+
+  (* TODO: move *)
+  Global Instance lm_ls_trans_dec st1 l st2:
+    Decision (lm_ls_trans LM st1 l st2).
+  Proof.
+    destruct l; simpl. 
+    3: { right. intros []. tauto. }
+    - solve_decision. 
+    - repeat apply and_dec; try solve_decision.
+      destruct (ls_tmap st1 (LM := LM) !! g) eqn:TMAP.
+      2: { right. intros [? MAP].
+           apply (ls_mapping_tmap_corr (LM := LM)) in MAP as (?&?&?).
+           set_solver. }
+      destruct (decide (g0 = ∅)) as [-> |NEMPTY].
+      { right. intros [? MAP].
+        apply (ls_mapping_tmap_corr (LM := LM)) in MAP as (?&?&?).
+        set_solver. }
+      left. apply set_choose_L in NEMPTY as [ρ ?].
+      exists ρ. apply (ls_mapping_tmap_corr (LM := LM)). eauto. 
+  Defined. 
+    
+  Definition allowed_step_FLs δ1 τ δ2: gset (@FairLabel G (fmrole M)) :=
+    filter (fun l => bool_decide (lm_ls_trans LM δ1 l δ2) = true)
+      (potential_step_FLs δ1 τ (LM := LM)).
+
+  Lemma aFLs_unique_TS_helper δ1 τ δ2 ρ:
+    Take_step ρ τ ∈ allowed_step_FLs δ1 τ δ2 ->
+    lm_ls_trans LM δ1 (Take_step ρ τ) δ2 /\ ls_mapping δ1 !! ρ = Some τ.
+  Proof.
+    rewrite /allowed_step_FLs /potential_step_FLs. 
+    rewrite !elem_of_filter. rewrite !elem_of_union.
+    rewrite elem_of_singleton elem_of_map.
+    intros [STEP%bool_decide_eq_true [[=] | IN]].
+    destruct IN as (?&[=]&?). subst.
+    split; auto.
+    apply STEP.
+  Qed.
+
+
+  Lemma locale_trans_alt δ1 τ δ2:
+    locale_trans δ1 τ δ2 <-> allowed_step_FLs δ1 τ δ2 ≠ ∅.
+  Proof using. 
+    rewrite /allowed_step_FLs /locale_trans. 
+    rewrite gset_not_elem_of_equiv_not_empty_L.
+    setoid_rewrite elem_of_filter.
+    rewrite /potential_step_FLs.
+    setoid_rewrite elem_of_union. setoid_rewrite elem_of_singleton.
+    setoid_rewrite elem_of_map. 
+    rewrite -ls_same_doms. setoid_rewrite elem_of_dom.  
+    setoid_rewrite bool_decide_eq_true. 
+    split.
+    - intros (ℓ & T & MATCH).
+      eexists. split; eauto.
+      destruct ℓ; simpl in MATCH; subst; try tauto.
+      right. eexists. split; eauto. inversion T. set_solver. 
+    - intros (?&STEP&POT).
+      destruct POT as [-> | (?&->&MAP)].
+      all: eexists; split; [eapply STEP| done]. 
+  Qed.
+
+  Global Instance locale_trans_dec st1 τ st2:
+    Decision (locale_trans st1 τ st2).
+  Proof.
+    eapply Decision_iff_impl; [symmetry; by apply locale_trans_alt| ].
+    solve_decision.
+  Qed.
+
+  (* TODO: move *)
+  Lemma iff_and_pre {A B C: Prop}
+    (BC: A -> (B <-> C)):
+    A /\ B <-> A /\ C.
+  Proof using. tauto. Qed.
+                    
+  Lemma aFLs_equiv ℓ δ1 τ δ2 :
+    ℓ ∈ allowed_step_FLs δ1 τ δ2 <-> lm_ls_trans LM δ1 ℓ δ2 /\ fair_lbl_matches_group ℓ τ.
+  Proof using.
+    rewrite /allowed_step_FLs elem_of_filter.
+    rewrite bool_decide_eq_true.
+    apply iff_and_pre. intros STEP. 
+    rewrite /potential_step_FLs /fair_lbl_matches_group.
+    rewrite elem_of_union elem_of_singleton elem_of_map.
+    split.
+    { by intros [-> | (?&->&?)]. } 
+    destruct ℓ; [..| done]; intros ->; eauto. 
+    right. eexists. split; eauto.
+    simpl in STEP. rewrite -ls_same_doms. apply elem_of_dom.
+    eexists. apply STEP. 
+  Qed. 
+
+End LocaleTrans. 
+
 (* excluding parts that are provided by other classes in context *)
 (* TODO: find a better solution *)
 Class LMFairPre' {G M LSI} (LM: LiveModel G M LSI) := {
@@ -12,6 +117,7 @@ Class LMFairPre' {G M LSI} (LM: LiveModel G M LSI) := {
   dTr' :> ∀ s1 ρ s2, Decision (fmtrans M s1 (Some ρ) s2);
   inhLM' :> Inhabited (lm_ls LM);
   inhG' :> Inhabited G;
+  locale_trans_ex_dec' τ δ1 :> Decision (exists δ2, locale_trans δ1 τ δ2 (LM := LM));
 }.
 
 Class LMFairPre {G M LSI} (LM: LiveModel G M LSI) := {
@@ -21,6 +127,7 @@ Class LMFairPre {G M LSI} (LM: LiveModel G M LSI) := {
   dTr :> ∀ s1 ρ s2, Decision (fmtrans M s1 (Some ρ) s2);
   inhLM :> Inhabited (lm_ls LM);
   inhG :> Inhabited G;
+  locale_trans_ex_dec τ δ1 :> Decision (exists δ2, locale_trans δ1 τ δ2 (LM := LM));
 }.
 
 
@@ -81,46 +188,6 @@ Section LMFair.
     set_solver. 
   Qed. 
 
-  Global Instance lm_ls_trans_dec st1 l st2:
-    Decision (lm_ls_trans LM st1 l st2).
-  Proof.
-    destruct l; simpl. 
-    3: { right. intros []. tauto. }
-    - solve_decision. 
-    - repeat apply and_dec; try solve_decision.
-      destruct (ls_tmap st1 (LM := LM) !! g) eqn:TMAP.
-      2: { right. intros [? MAP].
-           apply (ls_mapping_tmap_corr (LM := LM)) in MAP as (?&?&?).
-           set_solver. }
-      destruct (decide (g0 = ∅)) as [-> |NEMPTY].
-      { right. intros [? MAP].
-        apply (ls_mapping_tmap_corr (LM := LM)) in MAP as (?&?&?).
-        set_solver. }
-      left. apply set_choose_L in NEMPTY as [ρ ?].
-      exists ρ. apply (ls_mapping_tmap_corr (LM := LM)). eauto. 
-  Qed. 
-    
-  Definition potential_step_FLs (st1: lm_ls LM) (τ: G): 
-    gset (@FairLabel G (fmrole M)) :=
-    {[ Silent_step τ ]} ∪ (set_map (fun ρ => Take_step ρ τ) (dom (ls_fuel st1))).
-
-  Definition allowed_step_FLs δ1 τ δ2: gset (@FairLabel G (fmrole M)) :=
-    filter (fun l => bool_decide (lm_ls_trans LM δ1 l δ2) = true)
-      (potential_step_FLs δ1 τ).
-
-  Lemma aFLs_unique_TS_helper δ1 τ δ2 ρ:
-    Take_step ρ τ ∈ allowed_step_FLs δ1 τ δ2 ->
-    lm_ls_trans LM δ1 (Take_step ρ τ) δ2 /\ ls_mapping δ1 !! ρ = Some τ.
-  Proof.
-    rewrite /allowed_step_FLs /potential_step_FLs. 
-    rewrite !elem_of_filter. rewrite !elem_of_union.
-    rewrite elem_of_singleton elem_of_map.
-    intros [STEP%bool_decide_eq_true [[=] | IN]].
-    destruct IN as (?&[=]&?). subst.
-    split; auto.
-    apply STEP.
-  Qed.
-
   (* not true in general - it's possible to burn fuels even for the stepping role *)
   (* Lemma allowed_FLs_unique_TS δ1 τ δ2: *)
   (*   forall ρ1 ρ2, *)
@@ -128,49 +195,20 @@ Section LMFair.
   (*     Take_step ρ2 τ ∈ allowed_step_FLs δ1 τ δ2 -> *)
   (*     ρ1 = ρ2. *)
 
-  (* TODO: rename *)
-  Definition locale_trans (st1: lm_ls LM) (τ: G) st2 :=
-    exists ℓ, ls_trans (lm_fl LM) st1 ℓ st2 /\ fair_lbl_matches_group ℓ τ. 
-    
-  Lemma locale_trans_alt δ1 τ δ2:
-    locale_trans δ1 τ δ2 <-> allowed_step_FLs δ1 τ δ2 ≠ ∅.
-  Proof. 
-    rewrite /allowed_step_FLs /locale_trans. 
-    rewrite gset_not_elem_of_equiv_not_empty_L.
-    setoid_rewrite elem_of_filter.
-    rewrite /potential_step_FLs.
-    setoid_rewrite elem_of_union. setoid_rewrite elem_of_singleton.
-    setoid_rewrite elem_of_map. 
-    rewrite -ls_same_doms. setoid_rewrite elem_of_dom.  
-    setoid_rewrite bool_decide_eq_true. 
-    split.
-    - intros (ℓ & T & MATCH).
-      eexists. split; eauto.
-      destruct ℓ; simpl in MATCH; subst; try tauto.
-      right. eexists. split; eauto. inversion T. set_solver. 
-    - intros (?&STEP&POT).
-      destruct POT as [-> | (?&->&MAP)].
-      all: eexists; split; [eapply STEP| done]. 
-  Qed.
-
-  Global Instance locale_trans_dec st1 τ st2:
-    Decision (locale_trans st1 τ st2).
-  Proof.
-    eapply Decision_iff_impl; [symmetry; by apply locale_trans_alt| ].
-    solve_decision.
-  Qed.
-
-  Global Instance locale_trans_ex_dec τ δ1:
-    Decision (exists δ2, locale_trans δ1 τ δ2).
-  Proof.
-    set (fls := potential_step_FLs δ1 τ). 
-    (* destruct (decide ( *)
-    (* intros.  *)
-  Admitted.
+  (* Lemma lm_trans_simpl_dom δ1 ℓ δ2 *)
+  (*   (TRANS: lm_ls_trans LM δ1 ℓ δ2): *)
+  (*   exists (δ2': LiveState _ _ LSI), lm_ls_trans LM δ1 ℓ δ2 /\ *)
+  (*            ls_under δ2' = ls_under δ2 /\ ls_fuel δ2' = ls_fuel δ2 /\ *)
+  (*            ls_mapping δ2' = ls_mapping δ1. *)
+  (* Proof.  *)
+  (*   unshelve eset (δ2' := {| ls_under := ls_under δ2;  *)
+  (*                   ls_fuel := ls_fuel δ2; *)
+  (*                   ls_mapping := ls_mapping δ1 |}). *)
+  (*   { exact LSI. } *)
 
   Definition olocale_trans st1 oρ st2 :=
     match oρ with
-    | Some τ => locale_trans st1 τ st2
+    | Some τ => locale_trans st1 τ st2 (LM := LM)
     | _ => False
     end.
 
@@ -193,7 +231,7 @@ Section LMFair.
   Defined.
 
   Lemma LM_live_roles_strong δ τ:
-    τ ∈ live_roles LM_Fair δ <-> (exists δ', locale_trans δ τ δ').
+    τ ∈ live_roles LM_Fair δ <-> (exists δ', locale_trans δ τ δ' (LM := LM)).
   Proof.
     split.
     2: { intros [??]. eapply LM_Fair. simpl. eauto. }
@@ -201,12 +239,12 @@ Section LMFair.
   Qed.
 
   (* Useful in cases where the whole LM_Fair machinery cannot be used *)
-  Definition group_enabled τ δ := exists δ', locale_trans δ τ δ'.
+  Definition group_enabled τ δ := exists δ', locale_trans δ τ δ' (LM := LM).
 
   Lemma LM_live_role_map_notempty δ τ
     (LIVE: τ ∈ live_roles LM_Fair δ):
     exists R, ls_tmap δ (LM := LM) !! τ = Some R /\ R ≠ ∅.
-  Proof. 
+  Proof using.
     apply LM_live_roles_strong in LIVE as [? STEP].
     destruct STEP as (ℓ & T & MATCH).
     destruct ℓ; simpl in *; try done; subst. 
@@ -221,32 +259,10 @@ Section LMFair.
   Lemma LM_map_empty_notlive δ τ
     (MAP0: ls_tmap δ (LM := LM) !! τ = Some ∅ \/ ls_tmap δ (LM := LM) !! τ = None):
     τ ∉ live_roles LM_Fair δ. 
-  Proof. 
+  Proof using. 
     destruct (decide (τ ∈ live_roles LM_Fair δ)) as [LR| ]; [| done].
     apply LM_live_role_map_notempty in LR as (? & TMAP & NE).
     destruct MAP0; set_solver. 
   Qed. 
       
-  (* TODO: move *)
-  Lemma iff_and_pre {A B C: Prop}
-    (BC: A -> (B <-> C)):
-    A /\ B <-> A /\ C.
-  Proof using. tauto. Qed.
-                    
-  Lemma aFLs_equiv ℓ δ1 τ δ2 :
-    ℓ ∈ allowed_step_FLs δ1 τ δ2 <-> lm_ls_trans LM δ1 ℓ δ2 /\ fair_lbl_matches_group ℓ τ.
-  Proof using.
-    rewrite /allowed_step_FLs elem_of_filter.
-    rewrite bool_decide_eq_true.
-    apply iff_and_pre. intros STEP. 
-    rewrite /potential_step_FLs /fair_lbl_matches_group.
-    rewrite elem_of_union elem_of_singleton elem_of_map.
-    split.
-    { by intros [-> | (?&->&?)]. } 
-    destruct ℓ; [..| done]; intros ->; eauto. 
-    right. eexists. split; eauto.
-    simpl in STEP. rewrite -ls_same_doms. apply elem_of_dom.
-    eexists. apply STEP. 
-  Qed. 
-
 End LMFair.
